rustdemo/HashMapLink.v
@@ -1,0 +1,65 @@
+Require Import Coqlib.
+Require Import Errors.
+Require Import Maps.
+Require Import Integers.
+Require Import Floats.
+Require Import Values.
+Require Import AST.
+Require Import Values Globalenvs Memory.
+Require Import Events.
+Require Import Invariant Smallstep SmallstepLinkingSafe.
+Require Import LinkedList HashMap.
+Require Import HashMapCommon LinkedListSafe HashMapSafe.
+Require Import MoveCheckingDomain.
+Require Import InvariantAlgebra Compiler.
+
+Local Open Scope error_monad_scope.
+Local Open Scope inv_scope.
+Import ListNotations.
+
+(* The linked_list module (implemented in Rustlight) is totally safe
+after the compilation *)
+Lemma compiled_linked_list_safe: forall linked_list_asm,
+  transf_rustlight_program linked_list_mod = OK linked_list_asm ->
+  module_type_safe ((hmap_inv @@ rs_own) @! cc_rust_compcert) ((hmap_inv @@ rs_own) @! cc_rust_compcert) (Asm.semantics linked_list_asm) SIF.
+Proof.
+  intros.
+  eapply transf_rustlight_partial_safe_to_total_safe; eauto.
+  eapply linked_list_module_safe.
+Qed.
+
+(* The hash_map module is totally safe after the compilation *)
+Lemma compiled_hash_map_safe: forall hash_map_asm,
+  transf_clight_program hash_map_prog = OK hash_map_asm ->
+  module_type_safe ((hmap_inv @@ rs_own) @! cc_rust_compcert) ((hmap_inv @@ rs_own) @! cc_rust_compcert) (Asm.semantics hash_map_asm) SIF.
+Proof.
+  intros.
+  eapply open_safety_inv_ref.
+  3: { eapply transf_clight_total_safety_preservation. eauto.
+       eapply hash_map_module_safe. }
+  rewrite invcc_compose_assoc.
+  eapply cc_inv_ref. reflexivity.
+  eapply cc_rust_compcert_eqv.
+  red.
+  rewrite invcc_compose_assoc.
+  eapply cc_inv_ref. reflexivity.
+  eapply cc_rust_compcert_eqv.
+Qed.
+
+(** The semantically linked assembly module (linked_list_asm +
+hash_map_asm) is totally safe under the invariant ((hmap_inv @@
+rs_own) @! cc_rust_compcert). For now, the adequacy of Asm linking
+cannot be used to prove the safety of the syntactic linked module
+because it is a forward_simulation. *)
+Theorem link_linked_list_hash_map_safe: forall linked_list_asm hash_map_asm composed_sem,
+    transf_rustlight_program linked_list_mod = OK linked_list_asm ->
+    transf_clight_program hash_map_prog = OK hash_map_asm ->
+    SmallstepLinking.compose (Asm.semantics linked_list_asm) (Asm.semantics hash_map_asm) = Some composed_sem ->
+    module_type_safe ((hmap_inv @@ rs_own) @! cc_rust_compcert) ((hmap_inv @@ rs_own) @! cc_rust_compcert) composed_sem SIF.
+Proof.
+  intros.
+  eapply compose_total_type_safety; eauto.
+  eapply compiled_linked_list_safe; auto.
+  eapply compiled_hash_map_safe; auto.
+Qed.
+
